BF_Capflow高层实例化完成

BF_CapFlow.thy
@@ -4,6 +4,8 @@ imports Dynamic_model_v6 CapFlow_v6_0
 
 begin
 
+subsection {* Definitions *}
+
 subsubsection {* Data type, basic components, and state *}
 
 type_synonym systime_t = nat
@@ -53,6 +55,8 @@ datatype
             |ObjType_RAM
             |ObjType_PhysAddr
             |ObjType_Null
+
+datatype cap_state = DISTCAP_STATE_FOREIGN | DISTCAP_STATE_BUSY
 
 record dcb = disabled :: bool
              is_vm_guest :: bool
@@ -106,20 +110,21 @@ record DevFrame = base :: genpaddr_t
                   pasid :: pasid_t
                   bytes :: gensize_t
 
-datatype
-  capability_u =  PhysAddr 
-                 |RAM
-                 |L1CNode
-                 |L2CNode
-                 |FCNode
-                 |Dispatcher
-                 |EndPoint
-                 |Frame
-                 |DevFrame
+record capability_u =
+                  physaddr :: PhysAddr
+                  ram :: RAM
+                  l1cnode :: L1CNode
+                  l2cnode :: L2CNode
+                  fcnode :: FCNode
+                  dispatcher :: Dispatcher
+                  endpoint :: EndPoint
+                  frame :: Frame
+                  devframe :: DevFrame
 
 record capability = type :: objtype
                     rights :: right
                     union_of_cap :: capability_u
+                    state_of_cap :: cap_state
 
 record StateR = State + 
                 dispatchers :: "domain_id \<rightharpoonup> dcb"
@@ -140,10 +145,78 @@ definition abstract_state_rev :: "StateR \<Rightarrow> State \<Rightarrow> State
                             e_buf_size := e_buf_size r,
                             domain_endpoint := domain_endpoint r\<rparr>"
 
+datatype EventR = Client_Lookup_Endpoint_Name domain_id endpoint_name
+               | Send_Queuing_Message domain_id endpoint_id Message
+               | Receive_Queuing_Message domain_id endpoint_id
+               | Get_My_Endpoints_Set domain_id
+               | Get_Caps domain_id
+               | Grant_Endpoint_Cap domain_id cap cap
+               | Remove_Cap_Right domain_id cap right
+               | Sys_Dispatcher_Properties domain_id task_type systime_t systime_t systime_t nat systime_t
+               | Sys_Dispatcher_Setup domain_id cte lpaddr_t dispatcher_handle_t bool
+               | Dispatcher_Dump_Ptables domain_id
+               | Dispatcher_Dump_Capabilities domain_id
+               | Capability_Copy domain_id capability
+               | Capability_Retype domain_id capability objtype
+               | Capability_Mint domain_id capability nat nat
+               | Capability_Delete domain_id capability
+               | Capability_Get_State domain_id capability
+
 subsubsection {* Utility Functions used for Event Specification *} 
 
 
-subsubsection {* Events Definition *}
+subsubsection {* Events Specification *}
+
+definition client_lookup_endpoint_nameR :: "Sys_Config \<Rightarrow> StateR 
+              \<Rightarrow> domain_id \<Rightarrow> endpoint_name \<Rightarrow> (StateR \<times> endpoint_id option)" 
+  where "client_lookup_endpoint_nameR sc sr did ename \<equiv> 
+                                          let 
+                                            ret = (client_lookup_endpoint_name sc (\<Up>sr) did ename) 
+                                          in
+                                            (sr\<Down>(fst ret),snd ret)"
+
+definition send_queuing_messageR :: "StateR \<Rightarrow> domain_id \<Rightarrow> endpoint_id \<Rightarrow> Message \<Rightarrow> (StateR \<times> bool)"
+  where "send_queuing_messageR sr did eid m \<equiv>
+                                          let 
+                                            ret = (send_queuing_message (\<Up>sr) did eid m) 
+                                          in
+                                            (sr\<Down>(fst ret),snd ret)"
+
+definition receive_queuing_messageR :: "StateR \<Rightarrow> domain_id \<Rightarrow> endpoint_id \<Rightarrow> (StateR \<times> Message option)"
+  where "receive_queuing_messageR sr did eid \<equiv> 
+                                          let 
+                                            ret = (receive_queuing_message (\<Up>sr) did eid) 
+                                          in
+                                            (sr\<Down>(fst ret),snd ret)"
+
+definition get_my_endpoints_setR :: "StateR \<Rightarrow> domain_id \<Rightarrow> (StateR \<times> endpoint_id set)"
+  where "get_my_endpoints_setR sr did \<equiv> 
+                                  let 
+                                    ret = (get_my_endpoints_set (\<Up>sr) did) 
+                                  in
+                                    (sr\<Down>(fst ret),snd ret)"
+
+definition get_capsR :: "StateR \<Rightarrow> domain_id \<Rightarrow> (StateR \<times> cap set)"
+  where "get_capsR sr did \<equiv> 
+                      let 
+                        ret = (get_caps (\<Up>sr) did) 
+                      in
+                        (sr\<Down>(fst ret),snd ret)"
+
+definition grant_endpoint_capR :: "StateR \<Rightarrow> domain_id \<Rightarrow> cap \<Rightarrow> cap \<Rightarrow> (StateR \<times> bool)"
+  where "grant_endpoint_capR sr did grant_cap dst_cap \<equiv> 
+                      let 
+                        ret = (grant_endpoint_cap (\<Up>sr) did grant_cap dst_cap) 
+                      in
+                        (sr\<Down>(fst ret),snd ret)"
+
+definition remove_cap_rightR :: "StateR \<Rightarrow> domain_id \<Rightarrow> cap \<Rightarrow> right \<Rightarrow> (StateR
+ \<times> bool)"
+  where "remove_cap_rightR sr did rm_cap right_to_rm \<equiv> 
+                                          let 
+                                            ret = (remove_cap_right (\<Up>sr) did rm_cap right_to_rm) 
+                                          in
+                                            (sr\<Down>(fst ret),snd ret)"
 
 definition sys_dispatcher_properties :: "StateR \<Rightarrow> domain_id \<Rightarrow> task_type \<Rightarrow> systime_t  \<Rightarrow> systime_t 
                                         \<Rightarrow> systime_t \<Rightarrow> nat \<Rightarrow> systime_t \<Rightarrow> (StateR \<times> bool )" where
@@ -210,11 +283,13 @@ definition dispatcher_dump_capabilities :: "StateR \<Rightarrow> domain_id \<Rig
                                            in
                                             (sr\<Down>(fst ret),snd ret)"
 
+(*
 definition dispatcher_get_all_ep :: "StateR \<Rightarrow> domain_id \<Rightarrow> (StateR \<times> cap set )" where
   "dispatcher_get_all_ep sr did  \<equiv> let 
                                             ret = (get_caps (\<Up>sr) did) 
                                            in
                                             (sr\<Down>(fst ret),snd ret)"
+*)
 
 definition capability_copy :: "StateR \<Rightarrow> domain_id \<Rightarrow> capability \<Rightarrow> (StateR \<times> bool )" where
   "capability_copy sr did c \<equiv> 
@@ -246,12 +321,47 @@ definition capability_mint :: "StateR \<Rightarrow> domain_id \<Rightarrow> capa
                     c_space = cspaces sr;
                     c_set = c_space did;
                     c_set_rest =  {c. c\<in>c_set \<and> c\<noteq>cap_mint};
-                    target_union = union_of_cap cap_mint
+                    cap_u = union_of_cap cap_mint;
+                    cap_endpoint = endpoint cap_u;
+                    cap_endpoint_minted = cap_endpoint\<lparr>
+                      epoffset := param1,
+                      epbuflen := param2
+                    \<rparr>;
+                    cap_u_minted = cap_u\<lparr>
+                      endpoint := cap_endpoint_minted
+                    \<rparr>;
+                    cap_minted = cap_mint\<lparr>
+                      union_of_cap := cap_u_minted
+                    \<rparr>
                   in
-                    case target_union of
-                      (EndPoint) \<Rightarrow> (sr\<lparr>
-                      cspaces := c_space(did := insert cap_mint c_set_rest)
+                    if(type cap_mint = ObjType_EndPoint)
+                    then
+                      (sr
+                      \<lparr>
+                        cspaces := c_space(did := insert cap_minted c_set_rest)
+                      \<rparr>, True)
+                    else
+                      (sr, False)"
+
+definition capability_delete :: "StateR \<Rightarrow> domain_id \<Rightarrow> capability \<Rightarrow> (StateR \<times> bool )" where
+  "capability_delete sr did cap_del \<equiv> 
+                    let
+                    c_space = cspaces sr;
+                    c_set = c_space did;
+                    c_set_rest =  {c. c\<in>c_set \<and> c\<noteq>cap_del}
+                  in
+                    (sr
+                      \<lparr>
+                        cspaces := c_space(did := c_set_rest)
                       \<rparr>, True)"
+
+definition capability_get_state :: "StateR \<Rightarrow> domain_id \<Rightarrow> capability \<Rightarrow> (StateR \<times> cap_state )" where
+  "capability_get_state sr did cap_dst \<equiv> 
+                    let
+                    c_space = cspaces sr;
+                    c_set = c_space did
+                  in
+                    (sr, state_of_cap cap_dst)"
 
 definition system_initR :: "Sys_Config \<Rightarrow> StateR"
   where "system_initR sc \<equiv> let s0 = system_init sc in 
@@ -263,6 +373,24 @@ definition system_initR :: "Sys_Config \<Rightarrow> StateR"
                                 cspaces = (\<lambda> x. {})
                                \<rparr>"
 
+declare abstract_state_def[cong del] and abstract_state_rev_def[cong del] and 
+        client_lookup_endpoint_nameR_def [cong del] and 
+        send_queuing_messageR_def[cong del] and
+        receive_queuing_messageR_def[cong del] and
+        get_my_endpoints_setR_def[cong del] and
+        get_capsR_def[cong del] and
+        grant_endpoint_capR_def[cong del] and
+        remove_cap_rightR_def[cong del]
+
+declare abstract_state_def[cong] and abstract_state_rev_def[cong] and 
+        client_lookup_endpoint_nameR_def [cong ] and 
+        send_queuing_messageR_def[cong ] and
+        receive_queuing_messageR_def[cong ] and
+        get_my_endpoints_setR_def[cong ] and
+        get_capsR_def[cong ] and
+        grant_endpoint_capR_def[cong ] and
+        remove_cap_rightR_def[cong ]
+
 subsection{* Instantiation and Its Proofs of Security Model  *}
 
 consts s0r :: StateR
@@ -270,5 +398,206 @@ consts s0r :: StateR
 specification (s0r) 
   s0r_init: "s0r = system_initR sysconf"
   by simp
+
+definition exec_eventR :: "StateR \<Rightarrow> EventR \<Rightarrow> StateR" 
+  where "exec_eventR s e  \<equiv>
+    case e of  Client_Lookup_Endpoint_Name did ename 
+             \<Rightarrow> fst (client_lookup_endpoint_nameR sysconf s did ename)
+             | Send_Queuing_Message did eid m 
+             \<Rightarrow> fst (send_queuing_messageR s did eid m)
+             | Receive_Queuing_Message did eid 
+             \<Rightarrow> fst (receive_queuing_messageR s did eid)
+             | Get_My_Endpoints_Set did 
+             \<Rightarrow> fst (get_my_endpoints_setR s did)
+             | Get_Caps did 
+             \<Rightarrow> fst (get_capsR s did)
+             | Grant_Endpoint_Cap did grant_cap dst_cap 
+             \<Rightarrow> fst (grant_endpoint_capR s did grant_cap dst_cap)
+             | Remove_Cap_Right did dst_cap right_to_rm 
+             \<Rightarrow> fst (remove_cap_rightR s did dst_cap right_to_rm)
+             | Sys_Dispatcher_Properties did p_type p_deadline p_wcet p_period p_release p_weight
+             \<Rightarrow> fst (sys_dispatcher_properties s did p_type p_deadline p_wcet p_period p_release p_weight)
+             | Sys_Dispatcher_Setup did p_cptr p_vptr p_dptr p_run
+             \<Rightarrow> fst (sys_dispatcher_setup s did p_cptr p_vptr p_dptr p_run)
+             | Dispatcher_Dump_Ptables did 
+             \<Rightarrow> fst (dispatcher_dump_ptables s did)
+             | Dispatcher_Dump_Capabilities did 
+             \<Rightarrow> fst (dispatcher_dump_capabilities s did)
+             | Capability_Copy did c
+             \<Rightarrow> fst (capability_copy s did c)
+             | Capability_Retype did cap_retype dst_type
+             \<Rightarrow> fst (capability_retype s did cap_retype dst_type)
+             | Capability_Mint did cap_mint param1 param2
+             \<Rightarrow> fst (capability_mint s did cap_mint param1 param2)
+             | Capability_Delete did cap_del
+             \<Rightarrow> fst (capability_delete s did cap_del)
+             | Capability_Get_State did cap_dst
+             \<Rightarrow> fst (capability_get_state s did cap_dst)
+             "
+
+definition domain_of_eventR :: "EventR \<Rightarrow> domain_id option"
+  where "domain_of_eventR e \<equiv> 
+    case e of  Client_Lookup_Endpoint_Name did ename \<Rightarrow> Some did
+             | Send_Queuing_Message did eid m \<Rightarrow> Some did
+             | Receive_Queuing_Message did eid \<Rightarrow> Some did
+             | Get_My_Endpoints_Set did \<Rightarrow> Some did
+             | Get_Caps did \<Rightarrow> Some did
+             | Grant_Endpoint_Cap did grant_cap dst_cap \<Rightarrow> Some did
+             | Remove_Cap_Right did dst_cap right_to_rm  \<Rightarrow> Some did
+             | Sys_Dispatcher_Properties did p_type p_deadline p_wcet p_period p_release p_weight \<Rightarrow> Some did
+             | Sys_Dispatcher_Setup did p_cptr p_vptr p_dptr p_run \<Rightarrow> Some did
+             | Dispatcher_Dump_Ptables did \<Rightarrow> Some did 
+             | Dispatcher_Dump_Capabilities did \<Rightarrow> Some did 
+             | Capability_Copy did c \<Rightarrow> Some did
+             | Capability_Retype did cap_retype dst_type \<Rightarrow> Some did
+             | Capability_Mint did cap_mint param1 param2 \<Rightarrow> Some did
+             | Capability_Delete did cap_del \<Rightarrow> Some did
+             | Capability_Get_State did cap_dst \<Rightarrow> Some did
+              "
+
+definition vpeq_dispatcher :: "StateR \<Rightarrow> domain_id \<Rightarrow> StateR \<Rightarrow> bool" ("(_ \<sim>. _ .\<sim>\<^sub>\<Delta> _)")
+  where "vpeq_dispatcher s d t \<equiv> dispatchers s d = dispatchers t d
+                                 \<and> cspaces s d = cspaces t d" 
+
+lemma vpeq_dispatcher_transitive_lemma : 
+  "\<forall> s t r d. (vpeq_dispatcher s d t) \<and> (vpeq_dispatcher t d r) \<longrightarrow> (vpeq_dispatcher s d r)"
+  using vpeq_dispatcher_def by auto
+
+lemma vpeq_dispatcher_symmetric_lemma : "\<forall> s t d. (vpeq_dispatcher s d t) \<longrightarrow> (vpeq_dispatcher t d s)"
+  using vpeq_dispatcher_def by auto
+
+lemma vpeq_dispatcher_reflexive_lemma : "\<forall> s d. (vpeq_dispatcher s d s)"
+  using vpeq_dispatcher_def by auto
+
+definition vpeqR :: "StateR \<Rightarrow> domain_id \<Rightarrow> StateR \<Rightarrow> bool" ("(_ \<sim>. _ .\<sim> _)")
+  where "vpeqR s d t \<equiv>  ((\<Up>s) \<sim>d\<sim> (\<Up>t)) \<and> (s\<sim>.d.\<sim>\<^sub>\<Delta>t)"                         
+
+
+declare vpeqR_def[cong] and vpeq_dispatcher_def[cong]
+
+
+lemma vpeqR_transitive_lemma : "\<forall> s t r d. (vpeqR s d t) \<and> (vpeqR t d r) \<longrightarrow> (vpeqR s d r)"
+    apply(clarsimp cong del: vpeq1_def)
+    using vpeq1_transitive_lemma vpeq_dispatcher_transitive_lemma by blast
+
+lemma vpeqR_symmetric_lemma : "\<forall> s t d. (vpeqR s d t) \<longrightarrow> (vpeqR t d s)"
+  apply(clarsimp cong del: vpeq1_def)
+  using vpeq1_symmetric_lemma vpeq_dispatcher_symmetric_lemma by blast
+
+lemma vpeqR_reflexive_lemma : "\<forall> s d. (vpeqR s d s)"  
+  using vpeq1_reflexive_lemma vpeq_dispatcher_reflexive_lemma by auto
+
+lemma vpeqR_vpeq1 : "vpeqR s d t \<Longrightarrow> vpeq1 (\<Up>s) d (\<Up>t)"
+  using vpeqR_def by blast
+
+definition interferesR :: "domain_id \<Rightarrow> StateR \<Rightarrow> domain_id \<Rightarrow> bool"
+  where "interferesR w s v \<equiv> interferes w (\<Up>s) v"
+
+lemma interfR_reflexive_lemma : "\<forall>d s. interferesR d s d" 
+  using interferes_def interferesR_def by auto
+
+lemma policy_respectR_lemma : "\<forall>v u s t. (s \<sim>. u .\<sim>t)
+                              \<longrightarrow> (interferesR v s u = interferesR v t u)"
+  using interferesR_def vpeqR_def by auto
+
+lemma reachable_l2: "\<forall> s a. (SM.reachable0 s0r exec_eventR) s \<longrightarrow> (\<exists>s'. s' = exec_eventR s a)"
+  proof -
+  {
+    fix s a
+    assume p0: "(SM.reachable0 s0t exec_event) s"
+    have "(\<exists>s'. s' = exec_event s a)"
+      proof (induct a)
+        case (Client_Lookup_Endpoint_Name x) show ?case
+          apply (induct x)
+          by (simp add: exec_event_def) +
+        next
+        case (Send_Queuing_Message x1a x2 x3a) show ?case
+          apply (induct x1a)
+          by (simp add: exec_event_def) +
+        next
+        case (Receive_Queuing_Message x) show ?case
+          apply (induct x)
+          by (simp add: exec_event_def) +
+        next
+        case (Get_My_Endpoints_Set x) show ?case
+          apply (induct x)
+          by (simp add: exec_event_def) +
+        next
+        case (Get_Caps x ) show ?case
+          apply (induct x)
+          by (simp add: exec_event_def) +
+        case (Grant_Endpoint_Cap x1a x2 x3a ) show ?case
+          apply (induct x1a)
+          by (simp add: exec_event_def) +
+        case (Remove_Cap_Right x1a x2 ) show ?case
+          apply (induct x1a)
+          by (simp add: exec_event_def) +
+      qed
+    }
+  then show ?thesis by auto
+  qed
+
+interpretation SM_enabled 
+    s0r exec_eventR domain_of_eventR vpeqR interferesR
+   using vpeqR_transitive_lemma vpeqR_symmetric_lemma vpeqR_reflexive_lemma
+          interfR_reflexive_lemma policy_respectR_lemma reachable_l2
+          SM.intro[of vpeqR interferesR]
+          SM_enabled_axioms.intro[of s0r exec_eventR]
+          SM_enabled.intro[of vpeqR interferesR s0r exec_eventR] by blast
+
+subsection{* Proofs of refinement *}
+
+subsubsection{* Refinement of existing events at upper level *}
+
+lemma client_lookup_endpoint_name_ref_lemma: 
+    "\<forall>s. fst (client_lookup_endpoint_name sc (\<Up>s) did ename) 
+          = \<Up>(fst (client_lookup_endpoint_nameR sc s did ename))"
+    by auto
+
+lemma send_queuing_message_ref_lemma: 
+    "\<forall>s. fst (send_queuing_message (\<Up>sr) did eid m) 
+          = \<Up>(fst (send_queuing_messageR sr did eid m ))"
+    by auto
+
+lemma receive_queuing_message_ref_lemma: 
+    "\<forall>s. fst (receive_queuing_message (\<Up>sr) did eid) 
+            = \<Up>(fst (receive_queuing_messageR sr did eid))"
+    by auto
+
+lemma get_my_endpoints_set_ref_lemma: 
+    "\<forall>s. fst (get_my_endpoints_set (\<Up>sr) did) = \<Up>(fst (get_my_endpoints_setR sr did))"
+    by auto
+
+lemma get_caps_ref_lemma: 
+    "\<forall>s. fst (get_caps (\<Up>sr) did) = \<Up>(fst (get_capsR sr did))"
+    by auto
+
+lemma grant_endpoint_cap_ref_lemma: 
+    "\<forall>s. fst (grant_endpoint_cap (\<Up>sr) did grant_cap dst_cap) 
+              = \<Up>(fst (grant_endpoint_capR sr did grant_cap dst_cap))"
+    by auto
+
+lemma remove_cap_right_ref_lemma: 
+    "\<forall>s. fst (remove_cap_right (\<Up>sr) did rm_cap right_to_rm) 
+              = \<Up>(fst (remove_cap_rightR sr did rm_cap right_to_rm))"
+    by auto
+
+subsubsection{* new events introduced at this level dont change abstract state *}
+
+
+
+subsubsection{* proof of refinement *}
+
+  lemma s0_ref_lemma : "(\<Up>s0r) = s0t" 
+     by (simp add:  s0t_init s0r_init system_initR_def ) 
+
+
+subsection{* Existing events preserve "local respect" on new state variables *} 
+
+subsubsection{*proving "client lookup endpoint name"*}
+
+  lemma crt_smpl_portR_presrv_lcrsp_new:
+      assumes p3:"s' = fst (client_lookup_endpoint_nameR sc s did ename)"
+      shows   "s \<sim>. d .\<sim>\<^sub>\<Delta> s'" using p3 by fastforce    
 
 end
